Switching to FMap

RuntimeDefinitions.v
@@ -1,4 +1,12 @@
 From Coq Require Import Lists.List.
+From Coq Require Import FSets.FMapList.
+From Coq Require Import Structures.OrderedTypeEx.
+From Coq Require Import Structures.OrderedType.
+From Coq Require Import Init.Nat.
+From Coq Require Import Arith.Compare.
+Require Import Lia.
+
+Module Import NatMap := FMapList.Make(Nat_as_OT).
 
 (* Identifiers and Atomic Values *)
 Definition core_ID := nat.
@@ -10,7 +18,8 @@ Definition register_ID := nat.
 Definition raw_enclave_ID := nat.
 Definition data_offset := nat.
 Definition cache_tag_value := nat.
-Definition memory_address := nat.
+Inductive memory_address :=
+| address : block_ID -> data_offset -> memory_address.
 Definition instruction := nat.
 Definition number := nat.
 Definition process_ID := nat.
@@ -32,9 +41,7 @@ Inductive enclave_memory_range_value :=
 Inductive enclave_ID : Type :=
 | enclave_ID_active : raw_enclave_ID -> enclave_ID
 | enclave_ID_inactive : enclave_ID.
-Inductive enclave_memory_range_mapping := 
-| emr_mapping : raw_enclave_ID -> enclave_memory_range_value -> enclave_memory_range_mapping.
-Definition enclave_memory_range : Type := list enclave_memory_range_mapping.
+Definition enclave_memory_range : Type := NatMap.t enclave_memory_range_value.
 Inductive enclave_state : Type := 
 | enclave_state_value : enclave_ID -> enclave_memory_range -> enclave_state.
 
@@ -51,22 +58,105 @@ Inductive nullable_cachelet_index : Type :=
 | cachelet_index_none : nullable_cachelet_index.
 
 
-Inductive data_block_mapping :=
-| db_mapping : data_offset -> data -> data_block_mapping.
-Definition data_block := list data_block_mapping.
-Inductive remapping_mapping :=
-| remap_mapping : set_ID -> way_mask -> remapping_mapping.
-Definition remapping_list := list remapping_mapping.
 
+(*
+(* An ordered cachelet_index is needed *)
+Module cachelet_index_as_OT <: UsualOrderedType.
+  Definition t := cachelet_index.
+  Definition lt_ci (x: t) (y: t) : Prop :=
+  match x with
+  | cachelet_index_value w1 s1 =>
+    match y with
+    | cachelet_index_value w2 s2 => (lt w1 w2) \/ ((eq w1 w2) /\ (lt s1 s2))
+    end
+  end.
+  Definition eq_ci (x: t) (y: t) : Prop :=
+  match x with
+  | cachelet_index_value w1 s1 =>
+    match y with
+    | cachelet_index_value w2 s2 => (eq w1 w2) /\ (eq s1 s2)
+    end
+  end.
+  Definition eq := @eq t.
+  Definition eq_refl := @eq_refl t.
+  Definition eq_sym := @eq_sym t.
+  Definition eq_trans := @eq_trans t.
+  Definition lt := lt_ci.
+  Lemma lt_trans : forall x y z : t, lt x y -> lt y z -> lt x z.
+  Proof.
+    intros x y z H0 H1.
+    destruct x. destruct y. destruct z.
+    unfold lt in *. unfold lt_ci in *.
+    lia.
+  Qed.
+  Lemma lt_implies_not_eq : forall x y : nat, x < y -> x <> y.
+  Proof.
+    lia.
+  Qed.
+  Lemma eq_cachelet2 : forall x y z w: nat, x = z /\ y = w -> cachelet_index_value x y = cachelet_index_value z w.
+  Proof.
+    intros.
+    destruct H.
+    rewrite -> H.
+    rewrite -> H0.
+    auto.
+  Qed.
+  Lemma contrapositive : forall P Q : Prop, (P -> Q) -> (~Q -> ~P).
+  Proof. intros. intro. apply H0.  apply H. exact H1. Qed.
+  Lemma unequal_cachelet : forall x y z w: nat, x <> z \/ y <> w -> cachelet_index_value x y <> cachelet_index_value z w.
+  Proof.
+    intros.
+    specialize H.
+  Admitted.
+  Lemma eq_cachelet : forall x y z w : nat, cachelet_index_value x y = cachelet_index_value z w -> x = z /\ y = w.
+  Proof.
+    intros.
+    split.
+    induction x.
+    induction y.
+    induction z.
+    induction w.
+    auto. auto.
+    discriminate.
+    apply IHy.
+    rewrite <- H.
+  Admitted.
+  Lemma lt_not_eq : forall x y : t, lt x y -> ~ eq x y.
+  Proof.
+    intros x y H0.
+    destruct x. destruct y.
+    unfold eq.
+    unfold lt in H0. unfold lt_ci in H0.
+    destruct H0.
+    {
+      apply lt_implies_not_eq in H.
+      unfold not.
+      destruct eq.
+    }
+    lia.
+  Qed.
+  Definition compare x y := if x <=? y then (if y <=? x then Eq else Lt) else Gt.
+  Lemma eq_ci_dec : forall x y : t, {x = y} + {x <> y}.
+  Proof.
+    intros.
+    destruct x. destruct y.
+  Admitted.
+  Definition eq_dec := eq_ci_dec.
+End cachelet_index_as_OT.
+*)
+
+
+
+Definition data_block := NatMap.t data.
+Definition remapping_list := NatMap.t way_mask.
 (* Extra structure to hold data in way_set_cache *)
 Inductive way_set_cache_value : Type :=
 | valid_bit_tag_and_data : validity_bit -> cache_tag_value -> data_block -> way_set_cache_value.
 Inductive way_set_cache_mapping :=
 | wsc_mapping : cachelet_index -> way_set_cache_value -> way_set_cache_mapping.
 Definition way_set_cache := list way_set_cache_mapping.
-Inductive VPT_mapping :=
-| vpt_mapping : enclave_ID -> remapping_list -> VPT_mapping.
-Definition VPT := list VPT_mapping.
+(* NEED A MAP HERE *)
+Definition VPT := NatMap.t remapping_list.
 Definition CAT := list cachelet_index.
 
 
@@ -79,30 +169,20 @@ Inductive PLRU_leaf : Type :=
 Inductive PLRU_tree : Type :=
 | subtree : selection_bit -> enclave_ID -> PLRU_tree -> PLRU_tree -> PLRU_tree
 | subtree_leaf : PLRU_leaf -> PLRU_tree.
-Inductive set_indexed_PLRU_mapping :=
-| si_plru_mapping : set_ID -> PLRU_tree -> set_indexed_PLRU_mapping.
-Definition set_indexed_PLRU := list set_indexed_PLRU_mapping.
+Definition set_indexed_PLRU := NatMap.t PLRU_tree.
 
 
 (* Multi-Level Cache *)
 Inductive single_level_cache_unit : Type :=
 | single_level_cache : CAT -> VPT -> way_set_cache -> set_indexed_PLRU -> single_level_cache_unit.
-Inductive multi_level_cache_mapping :=
-| mlc_mapping : physical_cache_unit_ID -> single_level_cache_unit -> multi_level_cache_mapping.
-Definition multi_level_cache := list multi_level_cache_mapping.
+Definition multi_level_cache := NatMap.t single_level_cache_unit.
 
 
 (* Top-Level Structures *)
 Inductive process : Type :=
 | process_value : enclave_state -> memory_address -> core_ID -> process.
-Inductive process_mapping :=
-| p_mapping : process_ID -> process -> process_mapping.
-Definition processes := list process_mapping.
-Inductive register_mapping :=
-| reg_mapping : register_ID -> memory_value -> register_mapping.
-Definition registers := list register_mapping.
-Inductive memory_mapping :=
-| m_mapping : block_ID -> data_block -> memory_mapping.
-Definition memory := list memory_mapping.
+Definition processes := NatMap.t process.
+Definition registers := NatMap.t memory_value.
+Definition memory := NatMap.t data_block.
 Inductive runtime_state : Type :=
 | runtime_state_value : multi_level_cache -> memory -> registers -> processes -> runtime_state.
