AppendixE.v
@@ -4,34 +4,41 @@ From Coq Require Import Bool.Bool.
 From Coq Require Import Init.Nat.
 
 (* Checks if raw_enclave_ID is in the memory range for enclave_state *)
-Fixpoint contains_enclave (l: (list enclave_memory_range_mapping)) (id: raw_enclave_ID): bool :=
-  match l with
-  | nil => false
-  | x :: mem_range =>
-    match x with
-    | emr_mapping e _ =>
-      if eqb e id
-      then true
-      else contains_enclave mem_range id
-    end
+Definition contains_enclave (l: enclave_memory_range) (id: raw_enclave_ID): bool :=
+  match (NatMap.find id l) with
+  | Some x => true
+  | None => false
   end.
+Inductive validatable_enclave_state :=
+  | enclave_state_valid: enclave_state -> validatable_enclave_state
+  | enclave_state_error: validatable_enclave_state.
 
-(* Enclave Creation *)
+
+
 (*
-Definition enclave_creation (state: enclave_state) (mu: memory) (e: raw_enclave_ID) (l: memory_address) (n: data): enclave_state :=
+(* Enclave Creation *)
+Definition enclave_creation (state: enclave_state) (mu: memory) (e: raw_enclave_ID) (l: memory_address) (n: data): validatable_enclave_state :=
+  match state with
+  | enclave_state_value _ mem_range =>
+    if andb (negb (contains_enclave mem_range e)) (memory_currently_unallocated l n)
+    then enclave_state_error
+    else enclave_state_error
+  end.
 *)
-  
+
+
 
 (* Active Enclave Update *)
-Definition active_enclave_update (state: enclave_state) (id: enclave_ID): enclave_state :=
+Definition active_enclave_update (state: enclave_state) (id: enclave_ID): validatable_enclave_state :=
   match state with
   | enclave_state_value e mem_range =>
     match id with
     | enclave_ID_active x =>
-      if (contains_enclave mem_range x)
-      then enclave_state_value id mem_range
-      else state
-    | enclave_ID_inactive => enclave_state_value enclave_ID_inactive mem_range
+      match (contains_enclave mem_range x) with
+      | true => enclave_state_valid (enclave_state_value id mem_range)
+      | false => enclave_state_error
+      end
+    | enclave_ID_inactive => enclave_state_valid (enclave_state_value enclave_ID_inactive mem_range)
     end
   end.
 
@@ -45,7 +52,6 @@ Compute (active_enclave_update (enclave_state_value (enclave_ID_active 0) ((cons
   ++ (cons (emr_mapping 6 (enclave_address_and_data 0 data_none)) nil)
   ++ (cons (emr_mapping 2 (enclave_address_and_data 0 data_none)) nil))) (enclave_ID_active 1)).
 *)
-
 
 (* Enclave Elimination *)
 Fixpoint remove_enclave (id: raw_enclave_ID) (l: (list enclave_memory_range_mapping)): enclave_memory_range :=
